language_formal/spark2014_semantics/semantics.v
@@ -1,5 +1,6 @@
 Require Export values.
 Require Export environment.
+Require Import util.
 
 (** * Relational Semantics *)
 Definition eval_constant (cst: constant): return_val :=
@@ -29,52 +30,154 @@ Definition eval_unop (op: unary_operation) (v: return_val): return_val :=
     | Onot => Val.not v
     end.
 
+(* - - - - - - - - - - - - - - - - - - - - - - - - - - - - - - - - *)
+    
+(** ** Run-Time Checking Rules *)
+
+(** *** check actions *)
+(** which are needed to be performed before excecuting the program *)
+Inductive check_action: Type := 
+   | Division_Check: expr -> check_action
+   | Overflow_Check: expr -> check_action
+   | No_Check: check_action.
+
+(** *** semantics for check actions *)
+Inductive is_not_zero: Z -> bool -> Prop :=
+    | Not_Zero: forall v, v <> 0%Z -> is_not_zero v true
+    | Is_Zero: forall v, v = 0%Z -> is_not_zero v false.
+
+Definition Interpreter_Expr: Type := stack -> expr -> return_val -> Prop.
+
+Inductive do_check (IE: Interpreter_Expr): stack -> check_action -> bool -> Prop :=
+    | DC_Division_By_Zero: forall s e1 v1 e2 v2 b ast_id,
+        IE s e1 (ValNormal (Int v1)) -> (* make sure that v1 and v2 are type consistent *)
+        IE s e2 (ValNormal (Int v2)) ->
+        is_not_zero v2 b ->
+        do_check IE s (Division_Check (Ebinop ast_id Odiv e1 e2)) b
+    | DC_No_Check: forall s,
+        do_check IE s No_Check true.
+(*
+    | DC_Overflow: 
+    | DC_Range: 
+    | ... 
+*)
+
+(** *** check rules marking what and where to check *)
+(** 
+      - Do_Division_Check
+       
+       This flag is set on a division operator (/ mod rem) to indicate
+       that a zero divide check is required. 
+
+     - Do_Overflow_Check
+
+       This flag is set on an operator where an overflow check is required on
+       the operation. This flag is also set on if and case expression nodes if 
+       we are operating in either MINIMIZED or ELIMINATED overflow checking 
+       mode (to make sure that we properly process overflow checking for dependent 
+       expressions).
+*)
+
+Inductive check_flag: expr -> check_action -> Prop :=
+    | CF_Econst_Int: forall ast_id n,
+        check_flag (Econst ast_id (Ointconst n)) No_Check
+    | CF_Econst_Bool: forall ast_id b,
+        check_flag (Econst ast_id (Oboolconst b)) No_Check
+    | CF_Evar: forall ast_id x,  
+        check_flag (Evar ast_id x) No_Check
+    | CF_Ebinop_Div: forall ast_id e1 e2,
+        check_flag (Ebinop ast_id Odiv e1 e2) (Division_Check (Ebinop ast_id Odiv e1 e2))
+    | CF_Ebinop_Others: forall ast_id op e1 e2,
+        op <> Odiv ->
+        check_flag (Ebinop ast_id op e1 e2) No_Check
+    | CF_Eunop: forall ast_id op e,
+        check_flag (Eunop ast_id op e) No_Check.
+
+(** *** checking procedure *)
+Inductive run_time_check (IE: Interpreter_Expr):  stack -> expr -> bool -> Prop :=
+    | RTC: forall e runtime_check b s,
+        check_flag e runtime_check ->
+        do_check IE s runtime_check b ->
+        run_time_check IE s e b.
+
 (** ** Expression semantics *)
 Inductive eval_expr: stack -> expr -> return_val -> Prop :=
-    | eval_Econst: forall ast_id cst s v,
+    | eval_Econst: forall cst v s ast_id,
         eval_constant cst = v ->
         eval_expr s (Econst ast_id cst) v
-    | eval_Evar: forall ast_id v x s,
+    | eval_Evar: forall x s v ast_id,
         fetch x s = Some v ->
         eval_expr s (Evar ast_id x) (ValNormal v)
-    | eval_Ebinop: forall ast_id op s e1 e2 v1 v2 v,
-        eval_expr s e1 v1 ->
-        eval_expr s e2 v2 ->
-        eval_binop op v1 v2 = ValNormal v ->
-        eval_expr s (Ebinop ast_id op e1 e2) (ValNormal v)
-    | eval_Eunop: forall ast_id op s e v b,
-        eval_expr s e (ValNormal (Bool b)) ->
-        eval_unop op (ValNormal (Bool b)) = v ->
-        eval_expr s (Eunop ast_id op e) v.
+    | eval_Ebinop1: forall s e1 ast_id op e2,
+        eval_expr s e1 ValException ->
+        eval_expr s (Ebinop ast_id op e1 e2) ValException
+    | eval_Ebinop2: forall s e1 v1 e2 ast_id op,
+        eval_expr s e1 (ValNormal v1) ->
+        eval_expr s e2 ValException ->
+        eval_expr s (Ebinop ast_id op e1 e2) ValException
+    | eval_Ebinop3: forall s e1 v1 e2 v2 ast_id op,
+        eval_expr s e1 (ValNormal v1) ->
+        eval_expr s e2 (ValNormal v2) ->
+        run_time_check eval_expr s (Ebinop ast_id op e1 e2) false ->
+        eval_expr s (Ebinop ast_id op e1 e2) ValException
+    | eval_Ebinop4: forall s e1 v1 e2 v2 ast_id op v,
+        eval_expr s e1 (ValNormal v1) ->
+        eval_expr s e2 (ValNormal v2) ->
+        run_time_check eval_expr s (Ebinop ast_id op e1 e2) true ->
+        eval_binop op (ValNormal v1) (ValNormal v2) = v ->
+        v <> ValAbnormal ->
+        eval_expr s (Ebinop ast_id op e1 e2) v
+    | eval_Eunop1: forall s e ast_id op,
+        eval_expr s e ValException ->
+        eval_expr s (Eunop ast_id op e) ValException
+    | eval_Eunop2: forall s e v ast_id op v1,
+        eval_expr s e (ValNormal v) ->
+        eval_unop op (ValNormal v) = v1 ->
+        v1 <> ValAbnormal ->
+        eval_expr s (Eunop ast_id op e) v1.
+
 
 (** ** Command semantics *)
-Inductive eval_stmt: stack -> stmt -> stack -> Prop := 
-    | eval_Sassign: forall ast_id s s1 x e v,
+Inductive eval_stmt: stack -> stmt -> state -> Prop := 
+    | eval_Sassign1: forall s e ast_id x,
+        eval_expr s e ValException ->
+        eval_stmt s (Sassign ast_id x e) SException
+    | eval_Sassign2: forall s e v x s1 ast_id,
         eval_expr s e (ValNormal v) ->
         update s x (Value v) = Some s1 -> (* needs the type check on both sides *)
-        eval_stmt s (Sassign ast_id x e) s1
-    | eval_Sseq: forall ast_id s s1 s2 c1 c2,
-        eval_stmt s c1 s1 ->
+        eval_stmt s (Sassign ast_id x e) (SNormal s1)
+    | eval_Sseq1: forall s c1 ast_id c2,
+        eval_stmt s c1 SException ->
+        eval_stmt s (Sseq ast_id c1 c2) SException
+    | eval_Sseq2: forall ast_id s s1 s2 c1 c2,
+        eval_stmt s c1 (SNormal s1) ->
         eval_stmt s1 c2 s2 ->
         eval_stmt s (Sseq ast_id c1 c2) s2
-    | eval_Sifthen_True: forall ast_id s s1 b c,
+    | eval_Sifthen: forall s b ast_id c,
+        eval_expr s b ValException ->
+        eval_stmt s (Sifthen ast_id b c) SException
+    | eval_Sifthen_True: forall s b c s1 ast_id,
         eval_expr s b (ValNormal (Bool true)) ->
         eval_stmt s c s1 ->
         eval_stmt s (Sifthen ast_id b c) s1
-    | eval_Sifthen_False: forall ast_id s b c,
+    | eval_Sifthen_False: forall s b ast_id c,
         eval_expr s b (ValNormal (Bool false)) ->
-        eval_stmt s (Sifthen ast_id b c) s
-    | eval_Swhile_True: forall ast_id s s1 s2 b c,
+        eval_stmt s (Sifthen ast_id b c) (SNormal s)
+    | eval_Swhile: forall s b ast_id c,
+        eval_expr s b ValException ->
+        eval_stmt s (Swhile ast_id b c) SException
+    | eval_Swhile_True1: forall s b c ast_id,
         eval_expr s b (ValNormal (Bool true)) ->
-        eval_stmt s c s1 ->
+        eval_stmt s c SException ->
+        eval_stmt s (Swhile ast_id b c) SException
+    | eval_Swhile_True2: forall s b c s1 ast_id s2,
+        eval_expr s b (ValNormal (Bool true)) ->
+        eval_stmt s c (SNormal s1) ->
         eval_stmt s1 (Swhile ast_id b c) s2 ->
         eval_stmt s (Swhile ast_id b c) s2
-    | eval_Swhile_False: forall ast_id s b c,
+    | eval_Swhile_False: forall s b ast_id c,
         eval_expr s b (ValNormal (Bool false)) ->
-        eval_stmt s (Swhile ast_id b c) s.
-(*    | eval_Sassert: forall ast_id s e,
-        eval_expr s e (ValNormal (Bool true)) -> 
-        eval_stmt s (Sassert ast_id e) s. *)
+        eval_stmt s (Swhile ast_id b c) (SNormal s).
 
 (* - - - - - - - - - - - - - - - - - - - - - - - - - - - -  - - - - - - *)
 
@@ -87,20 +190,25 @@ Function f_eval_expr (s: stack) (e: expr): return_val :=
     | Evar _ x =>
         match (fetch x s) with  (* here we have not considered the variable's mode *)
         | Some v => ValNormal v
-        | None => ValException
+        | None => ValAbnormal
         end
     | Ebinop _ op e1 e2 =>
         match f_eval_expr s e1 with
         | ValNormal v1 => 
             match f_eval_expr s e2 with
             | ValNormal v2 => eval_binop op (ValNormal v1) (ValNormal v2)
-            | _ => ValException
+            | ValException => ValException
+            | ValAbnormal => ValAbnormal
             end
-        | _ => ValException
+        | ValException => ValException
+        | ValAbnormal => ValAbnormal
         end   
     | Eunop _ op e => 
-        let v := f_eval_expr s e in
-        eval_unop op v
+        match f_eval_expr s e with
+        | ValNormal v => eval_unop op (ValNormal v)
+        | ValException => ValException
+        | ValAbnormal => ValAbnormal
+        end
     end.
 
 (** ** Command semantics *)
@@ -114,21 +222,24 @@ Function f_eval_stmt k (s: stack) (c: stmt) {struct k}: state :=
         | ValNormal v => 
             match update s x (Value v) with
             | Some s1 => SNormal s1
-            | None => SException
+            | None => SAbnormal
             end
         | ValException => SException
+        | ValAbnormal => SAbnormal
         end
     | Sseq ast_id c1 c2 =>
         match f_eval_stmt k' s c1 with
         | SNormal s1 => f_eval_stmt k' s1 c2
         | SException => SException
         | SUnterminated => SUnterminated
+        | SAbnormal => SAbnormal
         end
     | Sifthen ast_id b c =>
         match f_eval_expr s b with
         | ValNormal (Bool true) => f_eval_stmt k' s c
         | ValNormal (Bool false) => SNormal s
-        | _ => SException
+        | ValException => SException
+        | _ => SAbnormal
         end
     | Swhile ast_id b c => 
         match f_eval_expr s b with
@@ -137,47 +248,247 @@ Function f_eval_stmt k (s: stack) (c: stmt) {struct k}: state :=
             | SNormal s1 => f_eval_stmt k' s1 (Swhile ast_id b c)
             | SException => SException
             | SUnterminated => SUnterminated
+            | SAbnormal => SAbnormal
             end
         | ValNormal (Bool false) => SNormal s
-        | _ => SException
+        | ValException => SException
+        | _ => SAbnormal
         end
     end
   end.
 
 (* - - - - - - - - - - - - - - - - - - - - - - - - - - - -  - - - - - - *)
+(** basic lemmas *)
+Lemma expr_type_infer: forall op v1 v2 n,
+    eval_binop op v1 v2 = ValNormal (Int n) -> 
+        (exists n1 n2, v1 = ValNormal (Int n1) /\ v2 = ValNormal (Int n2)).
+Proof.
+    intros.
+    unfold eval_binop in H. 
+    destruct v1 as [v1' | | ]; 
+    destruct v2 as [v2' | | ];
+    destruct op; 
+    simpl in H; try inversion H;
+    destruct v1'; 
+    destruct v2'; 
+    simpl in H; try inversion H;
+    try (exists n0, n1; auto).
+Qed.
 
-(** * Bisimulation Between Relational And Functional Semantics. *)
+Lemma expr_type_infer': forall op v1 v2 n,
+    eval_binop op v1 v2 = ValNormal (Bool n)  -> 
+        (exists n1 n2, v1 = ValNormal (Int n1) /\ v2 = ValNormal (Int n2)) \/ 
+        (exists n1 n2, v1 = ValNormal (Bool n1) /\ v2 = ValNormal (Bool n2)).
+Proof.
+    intros.
+    unfold eval_binop in H.
+    destruct v1 as [v1' | | ]; 
+    destruct v2 as [v2' | | ]; 
+    destruct op; 
+    simpl in H; try inversion H;
+    destruct v1'; 
+    destruct v2';
+    simpl in H; try inversion H.
+    left; exists n0, n1; auto.
+    left; exists n0, n1; auto.
+    right; exists b, b0; auto.
+    right; exists b, b0; auto.
+    left; exists n0, n1; auto.
+Qed.
+
+(* - - - - - - - - - - - - - - - - - - - - - - - - - - - -  - - - - - - *)
+
+(** * Bisimulation Between Relational And Functional Semantics *)
+
+Lemma eval_expr_unique: forall s e v1 v2,
+    eval_expr s e (ValNormal v1) ->
+    eval_expr s e (ValNormal v2) ->
+    v1 = v2.
+Proof.
+    induction e; 
+    intros v1 v2 h1 h2;
+    inversion h1; subst; 
+    inversion h2; subst.
+  - rewrite H3 in H4; inversion H4; subst.
+    auto.
+  - rewrite H1 in H2; inversion H2; auto.
+  - specialize (IHe1 _ _ H3 H4).
+    specialize (IHe2 _ _ H5 H10).
+    subst.
+    rewrite H13 in H8.
+    inversion H8; auto.
+  - specialize (IHe _ _ H1 H2).
+    subst.
+    destruct op, op0.
+    rewrite H6 in H3.
+    inversion H3; auto.
+Qed.
+
+Lemma eval_stmt_state : forall s p s',
+        eval_stmt s p s' ->                        (* s' is either a normal state or an exception *)
+            (exists v, s' = SNormal v) \/ s' = SException.
+Proof.
+    intros s p s' h.
+    induction h;
+    try match goal with
+    | [ |- (exists v, SNormal ?v1 = SNormal v) \/ _ ] => left; exists v1; reflexivity
+    | [ |- context [ _ \/ ?A = ?A ] ] => right; reflexivity
+    end; auto.
+Qed.
+
+Lemma Zeq_zero_true: forall v,
+    Zeq_bool v 0 = true <-> 
+    is_not_zero v false.
+Proof.
+    intros v.
+    split; intros h.
+  - apply Zeq_bool_eq in h.
+    constructor.
+    assumption.
+  - inversion h; subst.
+    auto.
+Qed.
+    
+Lemma Zeq_zero_false: forall v,
+    Zeq_bool v 0 = false <-> 
+    is_not_zero v true.
+Proof.
+    intros v.
+    split; intros h.
+  - apply Zeq_bool_neq in h.
+    constructor.
+    assumption.
+  - inversion h; subst.
+    destruct v; intuition.
+Qed.
+
+
 (** ** Semantics equivalence for expression *)
-Lemma f_eval_expr_correct : forall s e v,
+Lemma f_eval_expr_correct1 : forall s e v,
                         f_eval_expr s e = ValNormal v ->
                             eval_expr s e (ValNormal v).
 Proof.
     intros s e.
-    induction e; intros v h.
-  - (* 1. Econst *)
-    simpl in h; rewrite <- h.
-    constructor; reflexivity.
-  - (* 2. Evar *)
-    constructor.
-    simpl in h. destruct (fetch i s); try inversion h.
+    functional induction (f_eval_expr s e);
+    intros v0 h1;
+    try inversion h1; subst.
+  - constructor.
     reflexivity.
-  - (* 3. Ebinop *)
-    inversion h; subst.
-    remember (f_eval_expr s e1) as v1.
-    remember (f_eval_expr s e2) as v2.
-    destruct v1; destruct v2; try (inversion H0).
-    rewrite H0. econstructor; intuition.
-  - (* 4. Eunop *)
-    inversion h; subst.
-    unfold eval_unop in H0. destruct u.
-    remember (f_eval_expr s e) as v1.
-    destruct v1; try (inversion H0).
-    destruct v0; try (inversion H1).
-    subst.
-    specialize (IHe (Bool b)). intuition.
-    econstructor; intuition. assumption.
+  - constructor.
+    assumption.
+  - specialize (IHr _ e3).
+    specialize (IHr0 _ e4).
+    clear H0.
+    econstructor; auto; try assumption.
+    + (* check division by zero *)
+       destruct op;
+       match goal with
+       | [ |- run_time_check _ _ (Ebinop _ Odiv _ _) true ] => econstructor; [constructor | ]
+       | [ |- run_time_check _ _ (Ebinop _ _ _ _) true ] => econstructor; constructor; intuition; try inversion H
+       end.
+       destruct v1; destruct v2; simpl in h1; try inversion h1.
+       econstructor; intuition.
+       apply IHr.
+       apply IHr0.
+       remember (Zeq_bool n0 0) as eq.
+       destruct eq; try inversion h1.
+       symmetry in Heqeq.
+       apply Zeq_zero_false; assumption.
+    + rewrite h1. 
+       intuition. inversion H.
+  - specialize (IHr _ e2).
+    econstructor; intuition; try assumption.
+    rewrite h1 in H; inversion H.
 Qed.
 
+
+Lemma f_eval_expr_correct2 : forall s e,
+                        f_eval_expr s e = ValException ->
+                            eval_expr s e ValException.
+Proof.
+    intros s e.
+    functional induction (f_eval_expr s e);
+    intros h; try inversion h.
+  - destruct v; inversion h.
+  - rewrite h.
+    specialize (f_eval_expr_correct1 _ _ _ e3); intros hz1.
+    specialize (f_eval_expr_correct1 _ _ _ e4); intros hz2.
+    econstructor 5.
+    apply hz1. apply hz2.
+    destruct op;
+    destruct v1; destruct v2;
+    try inversion h.
+    econstructor. 
+    constructor.
+    econstructor. 
+    intuition.
+    apply hz1.
+    apply hz2.
+    remember (Zeq_bool n0 0) as eq.
+    symmetry in Heqeq.
+    destruct eq; try inversion h1.
+    apply Zeq_zero_true; assumption.
+    inversion H1.  
+  - specialize (IHr0 e4).
+    specialize (f_eval_expr_correct1 _ _ _ e3); intros hz1.
+    econstructor 4; auto.
+    apply hz1.
+  - specialize (IHr e3).
+    constructor; assumption.
+  - econstructor 8; intuition.
+    apply f_eval_expr_correct1; assumption.
+    repeat (progress constructor).
+    rewrite h in H. 
+    discriminate H.    
+  - specialize (IHr e2).
+    constructor; assumption.
+Qed.
+
+(** *** f_eval_expr_correct *)
+Lemma f_eval_expr_correct : forall s e v,
+                        (f_eval_expr s e = ValNormal v ->
+                            eval_expr s e (ValNormal v)) /\
+                        (f_eval_expr s e = ValException ->
+                            eval_expr s e ValException).
+Proof.
+    split.
+  - apply f_eval_expr_correct1.
+  - apply f_eval_expr_correct2.
+Qed.
+
+Lemma dividor_is_zero: forall s e2 v2 ast_id e1, 
+    eval_expr s e2 (ValNormal v2) ->
+    run_time_check eval_expr s (Ebinop ast_id Odiv e1 e2) false ->
+    v2 = Int 0.
+Proof.
+    intros.
+    inversion H0; subst.
+    inversion H1; subst.
+    inversion H2; subst.
+    specialize (eval_expr_unique _ _ _ _ H H9); intros hz1.
+    apply Zeq_zero_true in H10. 
+    apply Zeq_bool_eq in H10.
+    subst.
+    reflexivity.
+    intuition.
+Qed.
+
+(*
+Lemma dividor_is_zero: forall s e2 v2 ast_id e1, 
+    eval_expr s e2 (ValNormal (Int v2)) ->
+    run_time_check eval_expr s (Ebinop ast_id Odiv e1 e2) false ->
+    is_not_zero v2 false.
+Proof.
+    intros.
+    inversion H0; subst.
+    inversion H1; subst.
+    inversion H2; subst.
+    specialize (eval_expr_unique _ _ _ _ H H8); intros hz1.
+    rm_eq.
+Qed.
+*)
+
+(** *** f_eval_expr_complete *)
 Lemma f_eval_expr_complete : forall e s v,  
                         eval_expr e s v -> 
                             (f_eval_expr e s) = v.
@@ -189,15 +500,38 @@ Proof.
     | h: f_eval_expr _ _ = _ |- _ => progress rewrite h
     end;auto.
   - destruct v1; destruct v2;
-    [assumption | | | ]; 
-    destruct op in H; simpl in H; assumption.
+    destruct op;
+    inversion H; inversion H0; subst; inversion H1; 
+    subst; simpl; auto;
+    match goal with
+    | [h1: eval_expr ?s e1 (ValNormal ?v1), h2: eval_expr ?s e1 (ValNormal ?v1') |- _ ] =>
+            specialize (eval_expr_unique _ _ _ _  h1 h2); let hz := fresh "hz" in intros hz; inversion hz; subst
+    end;
+    match goal with
+    | [h1: eval_expr ?s e2 (ValNormal ?v2), h2: eval_expr ?s e2 (ValNormal ?v2') |- _ ] =>
+            specialize (eval_expr_unique _ _ _ _  h1 h2); let hz := fresh "hz" in intros hz; inversion hz; subst
+    end;
+    match goal with
+    | [h1: eval_expr _ ?e2 (ValNormal ?v2), h2: run_time_check _ _ (Ebinop _ Odiv _ ?e2) false |- _ ] =>
+            specialize (dividor_is_zero _ _ _ _ _ h1 h2); let hz := fresh "hz" in intros hz; inversion hz; subst; simpl; auto
+    end.
 Qed.
 
 
 Ltac blam :=
   match goal with
-    | H:SUnterminated _ = SNormal _ |- _ => inversion H
+    | H:SUnterminated = SNormal _ |- _ => inversion H
+    | H:SUnterminated = SException |- _ => inversion H
+    | H:SUnterminated = SAbnormal |- _ => inversion H
+    | H:SAbnormal = SNormal _ |- _ => inversion H
+    | H:SAbnormal = SException |- _ => inversion H
+    | H:SAbnormal = SUnterminated |- _ => inversion H
     | H:SException = SNormal _ |- _ => inversion H
+    | H:SException = SAbnormal |- _ => inversion H
+    | H:SException = SUnterminated |- _ => inversion H
+    | H:SNormal _ = SUnterminated |- _ => inversion H
+    | H:SNormal _ = SException |- _ => inversion H
+    | H:SNormal _ = SAbnormal |- _ => inversion H
     | H:SNormal _ = SNormal _ |- _ => inversion H;clear H;subst 
     | h:update _ _ (Value _) = _ |- _ => rewrite h
     | H : f_eval_stmt _ _ _ = _ |- _ => rewrite H
@@ -208,27 +542,56 @@ Ltac invle := match goal with
     | H: (S _ <= _)%nat |- _ => (inversion H; clear H; subst;simpl)
   end.
 
-Lemma f_eval_stmt_fixpoint: forall s p (k:nat) s', 
+Lemma f_eval_stmt_fixpoint: forall k s p s', 
         f_eval_stmt k s p = SNormal s' ->
         forall k':nat, (k <= k')%nat -> 
             f_eval_stmt k' s p = SNormal s'.
 Proof.
-    intros s p k.
+    intros k s p.
     functional induction (f_eval_stmt k s p); simpl; intros; subst; simpl; auto;
     repeat progress blam.
-  - inversion H.
   - invle.
     + repeat blam.
     + blam. blam.
   - invle.
     + repeat blam.
     + rewrite (IHs0 _ e1);auto with arith.
-  - inversion H.
   - invle; repeat blam. rewrite (IHs0 _ H);auto with arith.
   - invle; repeat blam.
   - invle; repeat blam. rewrite (IHs0 _ e2); auto with arith.
-  - inversion H.
   - invle; repeat blam.
+Qed.
+
+Lemma f_eval_stmt_fixpoint_E: forall k s p, 
+        f_eval_stmt k s p = SException ->
+        forall k':nat, (k <= k')%nat -> 
+            f_eval_stmt k' s p = SException.
+Proof.
+    intros k s p.
+    functional induction (f_eval_stmt k s p); simpl; intros; subst; simpl; auto;
+    repeat progress blam. 
+  - invle;
+    blam.
+  - invle;
+    repeat blam.
+    rewrite (f_eval_stmt_fixpoint _ _ _ _ e1); auto with arith.
+  - invle;
+    repeat blam.
+    specialize (IHs0 e1). 
+    rewrite IHs0; auto with arith. 
+  - invle; 
+    repeat blam.
+    rewrite IHs0; auto with arith.
+  - invle;
+    repeat blam.
+  - invle; 
+    repeat blam. 
+    rewrite (f_eval_stmt_fixpoint _ _ _ _ e2); auto with arith.
+  - invle; 
+    repeat blam.
+    rewrite (IHs0 e2); auto with arith.    
+  - invle; 
+    repeat blam.   
 Qed.
 
 
@@ -246,118 +609,178 @@ Ltac kgreater :=
              rewrite (@f_eval_stmt_fixpoint _ _ _ _ h);auto with arith
            | h:f_eval_stmt ?k ?s ?p = SNormal ?s' |- context [f_eval_stmt (_ + ?k) ?s ?p] =>
              rewrite (@f_eval_stmt_fixpoint _ _ _ _ h);auto with arith
+           | h:f_eval_stmt ?k ?s ?p = SException |- context [f_eval_stmt (?k + _) ?s ?p] =>
+             rewrite (@f_eval_stmt_fixpoint_E _ _ _ h);auto with arith
+           | h:f_eval_stmt ?k ?s ?p = SException |- context [f_eval_stmt (_ + ?k) ?s ?p] =>
+             rewrite (@f_eval_stmt_fixpoint_E _ _ _ h);auto with arith
          end.
 
 (** ** Semantics equivalence for command *)
 
-Lemma f_eval_stmt_correct : forall k s p s',
+Ltac rm_f_eval_expr :=
+    match goal with 
+    | [ h: f_eval_expr ?s ?b = ValException |- _ ] => specialize (f_eval_expr_correct2 _ _ h); intros hz1
+    | [ h: f_eval_expr ?s ?b = ValNormal ?v |- _ ] => specialize (f_eval_expr_correct1 _ _ _ h); intros hz1   
+(*
+    | [ h: f_eval_stmt ?k ?s ?c = SException |- _ ] => specialize (f_eval_stmt_correct1 _ _ _ _ h); intros hz1
+    | [ h: f_eval_stmt ?k ?s ?c = SNormal ?s1 |- _ ] => specialize (f_eval_stmt_correct1 _ _ _ _ h); intros hz1
+*)
+    end; auto.
+
+Lemma f_eval_stmt_correct1 : forall k s p s',
         f_eval_stmt k s p = SNormal s' ->
-          eval_stmt s p s'.
+          eval_stmt s p (SNormal s').
 Proof.
     intros k s p.
-    functional induction (f_eval_stmt k s p); 
-    intros s' H; try inversion H.
+    functional induction (f_eval_stmt k s p);
+    intros s' H; try inversion H; subst.
   - (* Sassign *)
-    eapply eval_Sassign. 
-    apply f_eval_expr_correct in e2. apply e2.
-    blam.
+    econstructor.
+    rm_f_eval_expr.
+    apply hz1.
+    assumption.
   - (* Sseq *)
-    eapply eval_Sseq. 
-    specialize (IHs0 s1 e1).
-    apply IHs0. 
-    specialize (IHs1 s' H).
-    apply IHs1.
+    specialize (IHs0 _ e1).
+    specialize (IHs1 _ H).
+    econstructor.
+    apply IHs0.
+    blam.
   - (* Cifthen_True *)
-    eapply eval_Sifthen_True.
-    apply f_eval_expr_correct in e1. assumption.
-    specialize (IHs0 s' H). assumption.
+    specialize (IHs0 _ H).
+    econstructor.
+    rm_f_eval_expr. 
+    blam.
   - (* Cifthen_False *)
     eapply eval_Sifthen_False.
-    apply f_eval_expr_correct in e1. 
-    subst. assumption.
+    rm_f_eval_expr.
   - (* Swhile_True *)
-    eapply eval_Swhile_True.
-    apply f_eval_expr_correct in e1. assumption.
-    specialize (IHs0 s1 e2). apply IHs0.
-    specialize (IHs1 s' H). assumption.
+    specialize (IHs0 _ e2).
+    specialize (IHs1 _ H).
+    econstructor.
+    rm_f_eval_expr.
+    apply IHs0. 
+    blam.
   - (* Swhile_False *)
     eapply eval_Swhile_False.
-    apply f_eval_expr_correct in e1. 
-    subst; assumption.
+    rm_f_eval_expr.
 Qed.
 
+Ltac rm_f_eval_stmt :=
+    match goal with 
+    | [ h: f_eval_stmt ?k ?s ?c = SNormal ?s1 |- _ ] => specialize (f_eval_stmt_correct1 _ _ _ _ h); intros hz1
+    end; auto.
 
-Lemma f_eval_stmt_complete : forall s p s',
-        eval_stmt s p s' ->
-            exists k, f_eval_stmt k s p = SNormal s'.
+Lemma f_eval_stmt_correct2 : forall k s p,
+        f_eval_stmt k s p = SException ->
+          eval_stmt s p SException.
 Proof.
-  intros s p s' H.
-  induction H.
+    intros k s p.
+    functional induction (f_eval_stmt k s p);
+    intros H; try inversion H; subst.
+  - (* Sassign *)
+    econstructor.
+    rm_f_eval_expr.
+  - (* Sseq *)
+    specialize (IHs1 H).
+    econstructor.
+    rm_f_eval_stmt.
+    apply hz1.
+    blam.
+  - specialize (IHs0 e1).
+    econstructor.
+    assumption.    
+  - (* Cifthen *)
+    specialize (IHs0 H).
+    econstructor.
+    rm_f_eval_expr.
+    blam.
+  - econstructor.
+    specialize (f_eval_expr_correct2 _ _ e1); intros hz1. 
+    assumption.
+  - (* Swhile *)
+    specialize (IHs1 H).
+    econstructor.
+    rm_f_eval_expr.
+    rm_f_eval_stmt.
+    apply hz1.
+    blam.
+  - constructor 9.
+    rm_f_eval_expr.
+    specialize (IHs0 e2); assumption.    
+  - econstructor.
+    rm_f_eval_expr.
+Qed.
+
+Ltac rm_f_eval :=
+    match goal with 
+    | [ h: f_eval_expr ?s ?b = ValException |- _ ] => specialize (f_eval_expr_correct2 _ _ h); intros hz1
+    | [ h: f_eval_expr ?s ?b = ValNormal ?v |- _ ] => specialize (f_eval_expr_correct1 _ _ _ h); intros hz1   
+    | [ h: f_eval_stmt ?k ?s ?c = SException |- _ ] => specialize (f_eval_stmt_correct2 _ _ _ h); intros hz1
+    | [ h: f_eval_stmt ?k ?s ?c = SNormal ?s1 |- _ ] => specialize (f_eval_stmt_correct1 _ _ _ _ h); intros hz1
+    end; auto.
+
+(** *** f_eval_stmt_correct *)
+Lemma f_eval_stmt_correct : forall k s p s',
+        (f_eval_stmt k s p = SNormal s' ->
+          eval_stmt s p (SNormal s')) /\ 
+        (f_eval_stmt k s p = SException ->
+          eval_stmt s p SException).
+Proof.
+    intros.
+    split; intros;
+    rm_f_eval.
+Qed.
+
+(** *** f_eval_stmt_complete *)
+Lemma f_eval_stmt_complete : forall s p s',
+        eval_stmt s p s' ->                        (* s' is either a normal state or an exception *)
+            exists k, f_eval_stmt k s p = s'.
+Proof. 
+  intros s p s' H;
+  induction H;
+  try match goal with
+  [ h: eval_expr ?s ?e ValException |- exists k, _ = SException] => 
+          exists 1%nat; simpl;
+          rewrite (f_eval_expr_complete _ _ _ h);
+          reflexivity
+  end.
+  (* 1. Sassign *)
   - exists 1%nat. simpl.
     rewrite (f_eval_expr_complete _ _ _ H).
-    rewrite H0. 
-    reflexivity.
+    blam.   
+  (* 2. Sseq *)
   - destrIH.
-    exists (S (k0+k)).
-    simpl.
+    exists (S k); simpl.
+    blam.
+  - destrIH.
+    exists (S (k0+k)); simpl.
     kgreater.
+    specialize (eval_stmt_state _ _ _ H0); intros hz1.
+    destruct hz1 as [hz2 | hz2]; try rm_exists; subst;
+    kgreater.
+  (* 3. Sifthen *)
   - destrIH.
-    exists (S (k)).
-    simpl.
+    exists (S k); simpl.
     rewrite (f_eval_expr_complete _ _ _ H).
     assumption.
-  - exists (S 0).
-    simpl.
+  - exists 1%nat. simpl.
     rewrite (f_eval_expr_complete _ _ _ H).
     reflexivity.
+  (* 4. Swhile *)
   - destrIH.
-    exists (S (k0+k)).
-    simpl.
+    exists (S k); simpl.
+    rewrite (f_eval_expr_complete _ _ _ H).
+    blam.
+  - destrIH.
+    exists (S (k0+k)); simpl.
+    rewrite (f_eval_expr_complete _ _ _ H).    
     kgreater.
+    specialize (eval_stmt_state _ _ _ H1); intros hz1.
+    destruct hz1 as [hz2 | hz2]; try rm_exists; subst;
+    kgreater.
+  - exists 1%nat. simpl.
     rewrite (f_eval_expr_complete _ _ _ H).
     reflexivity.
-  - exists (S 0).
-    simpl.
-    rewrite (f_eval_expr_complete _ _ _ H).
-    reflexivity.
-Qed.
-    
-
-(* - - - - - - - - - - - - - - - - - - - - - - - - - - - -  - - - - - - *)
-(** basic lemmas *)
-Lemma expr_type_infer: forall op v1 v2 n,
-    eval_binop op v1 v2 = ValNormal (Int n) -> (exists n1 n2, v1 = ValNormal (Int n1) /\ v2 = ValNormal (Int n2)).
-Proof.
-    intros.
-    unfold eval_binop in H. 
-    destruct v1 as [v1' | ]; 
-    destruct v2 as [v2' | ];
-    destruct op; 
-    simpl in H; try inversion H;
-    destruct v1'; 
-    destruct v2'; 
-    simpl in H; try inversion H;
-    try (exists n0, n1; auto).
-Qed.
-
-Lemma expr_type_infer': forall op v1 v2 n,
-    eval_binop op v1 v2 = ValNormal (Bool n)  -> 
-        (exists n1 n2, v1 = ValNormal (Int n1) /\ v2 = ValNormal (Int n2)) \/ 
-        (exists n1 n2, v1 = ValNormal (Bool n1) /\ v2 = ValNormal (Bool n2)).
-Proof.
-    intros.
-    unfold eval_binop in H.
-    destruct v1 as [v1' | ]; 
-    destruct v2 as [v2' | ]; 
-    destruct op; 
-    simpl in H; try inversion H;
-    destruct v1'; 
-    destruct v2';
-    simpl in H; try inversion H.
-    left; exists n0, n1; auto.
-    left; exists n0, n1; auto.
-    right; exists b, b0; auto.
-    right; exists b, b0; auto.
 Qed.
 
 
