language_formal/spark2014_semantics/util.v
@@ -1,36 +1,31 @@
-Require Export wellformed.
-
 (** * Customized Tactics *)
 
-Ltac rm_eval_expr :=
-    repeat match goal with
-    | [ |- eval_expr _ (Evar _ _) _] => apply eval_Evar
-    | [ |- eval_expr ?S (Ebinop _ _ _ _) _] => eapply eval_Ebinop
-    | [h: eval_expr ?S ?E ?V |- eval_expr ?S ?E _] => apply h 
-    | [h: eval_binop ?OP _ _  = ?V |- eval_binop ?OP _ _ = ?V ] => apply h
-    | [h: ?A |- ?A] => apply h
-    end.
-
-Ltac simpl_unop := 
+Ltac simpl_unop unfunc := 
     match goal with
-    | [ |- context[eval_unop ?uop (ValNormal (Bool ?b))]] => unfold eval_unop; simpl
+    | [ |- context[unfunc ?uop (_ (_ ?b))]] => unfold unfunc; simpl
     end.
 
-Ltac simpl_binop :=
+Ltac simpl_binop binfunc :=
     match goal with
-    | [ |- context [eval_binop ?OP (ValNormal ?V1) (ValNormal ?V2)]] => unfold eval_binop; simpl
+    | [ |- context [binfunc ?OP (_ ?V1) (_ ?V2)]] => unfold binfunc; simpl
     end.
 
-Ltac simpl_binop_hyp :=
+(* this for operation on type system *)
+Ltac simpl_binop_hyp1 binfunc  :=
     repeat match goal with
-    | [h: Some ?T = binop_type ?OP ?T1 ?T1 |- _ ] => 
-            unfold binop_type in h; simpl in h; inversion h; subst
-    | [h: binop_type ?OP ?T1 ?T1 = Some ?T |- _ ] => 
-            unfold binop_type in h; simpl in h; inversion h; subst
-    | [h: ValNormal ?V = eval_binop ?OP (ValNormal _) (ValNormal _) |- _] =>
-            unfold eval_binop in h; simpl in h; inversion h; subst
-    | [h: eval_binop ?OP (ValNormal _) (ValNormal _) = ValNormal ?V |- _] =>
-            unfold eval_binop in h; simpl in h; inversion h; subst
+    | [h: Some ?T = binfunc ?OP ?T1 ?T1 |- _ ] => 
+            unfold binfunc in h; simpl in h; inversion h; subst
+    | [h: binfunc ?OP ?T1 ?T1 = Some ?T |- _ ] => 
+            unfold binfunc in h; simpl in h; inversion h; subst
+    end.
+
+(* this is for operation on values *)
+Ltac simpl_binop_hyp2 binfunc  :=
+    repeat match goal with
+    | [h: ?ValNormal ?V = binfunc ?OP (?ValNormal _) (?ValNormal _) |- _] =>
+            unfold binfunc in h; simpl in h; inversion h; subst
+    | [h: binfunc ?OP (?ValNormal _) (?ValNormal _) = ?ValNormal ?V |- _] =>
+            unfold binfunc in h; simpl in h; inversion h; subst
     end.
 
 Ltac specialize_hypo := 
@@ -39,30 +34,13 @@ Ltac specialize_hypo :=
     | [h: ?A, h1: ?A -> _ -> _ |- _] => specialize (h1 h)
     end.
 
-Ltac rm_wt_expr :=
-    repeat match goal with
-    | [ |- well_typed_expr _ (Evar _ _) _] => apply WT_Evar
-    | [ |- well_typed_expr _ (Eunop _ _ _) _] => eapply WT_Eunop
-    | [ |- well_typed_expr _ (Ebinop _ ?OP ?E1 ?E2) ?T] => eapply WT_Ebinop (* it will generate some universal variables *)
-    | [ h: well_typed_expr _ ?E ?T |- well_typed_expr _ ?E _ ] => apply h 
-    | [ |- context[binop_type _ _ _]] => unfold binop_type; auto
-    end.
-
-(*
-Ltac rm_wd_expr :=
-    repeat match goal with
-    | [ |- well_defined_expr _ (Econst _ ?C)] => destruct C; apply (WD_Econst_Bool, WD_Econst_Int)
-    | [ |- well_defined_expr _ (Evar _ _)] => eapply WD_Evar;
-          match goal with 
-          [ h: fetch ?X ?S = Some ?V |- fetch ?X ?S = Some _ ] => apply h
-          end
-    | [ |- well_defined_expr ?S (Ebinop _ ?OP ?E1 ?E2)] => apply WD_Ebinop; specialize_hypo; assumption
-    | [ |- well_defined_expr ?S (Eunop _ ?OP ?E)] => apply WD_Eunop; specialize_hypo; assumption
-    | [ h: fetch ?X ?S = Some ?V |- well_defined_expr ?S (Evar _ ?X)] => destruct V; subst
-    end.
-*)
 
 (* - - - - - - - - - - - - - - - - - - - - - - - - - - - - - - - - - - - *)
+
+Ltac rm_eq :=
+    match goal with
+    [h: ?A _ = ?A _ |- _] => inversion h as [h1]; auto
+    end.
 
 Ltac put_in_context_as hname :=
     match goal with
