language_formal/spark2014_semantics/wellformedness.v
@@ -1,0 +1,979 @@
+Require Export environment.
+Require Export semantics.
+
+(** * Well-Formed Program  *)
+(**
+   Before executing the program, make sure that the program is well-formed
+   - well-typed
+      - all operators work on the operands of the right types;
+      - all assignments write into memory with the values of right types;
+      - variables has right _in/out_ mode;
+   - well-defined 
+      - all variables are initialized before they are used
+   - well-checked
+      - right checks are put at the right places
+*)
+
+Definition binop_type (op: binary_operation) (x y: typ): option typ := 
+    match op with 
+    | Ceq | Cne  => 
+        match x, y with
+        | Tint, Tint => Some Tbool
+        | _, _ => None
+        end
+    | Oand | Oor =>
+        match x, y with
+        | Tbool, Tbool => Some Tbool
+        | _, _ => None
+        end
+    | Oadd | Osub | Omul | Odiv =>
+        match x, y with
+        | Tint, Tint => Some Tint
+        | _, _ => None
+        end
+    end.
+
+(** * Well-Typed *)
+(** ** Well-typed expressions *)
+(**
+   - general type checking;
+   - all variables should be in mode _in_; 
+*)
+Inductive well_typed_expr: symtb -> expr -> typ -> Prop :=
+    | WT_Econst_Int: forall ast_id n tb,
+        well_typed_expr tb (Econst ast_id (Ointconst n)) Tint
+    | WT_Econst_Bool: forall ast_id b tb,
+        well_typed_expr tb (Econst ast_id (Oboolconst b)) Tbool
+    | WT_Evar: forall ast_id x tb t,
+        lookup x tb = Some (In, t) ->  (* the 'out' variables can never be read *)    
+        well_typed_expr tb (Evar ast_id x) t
+    | WT_Ebinop: forall ast_id tb op e1 e2 t t1,
+        well_typed_expr tb e1 t ->
+        well_typed_expr tb e2 t ->
+        binop_type op t t = Some t1 ->
+        well_typed_expr tb (Ebinop ast_id op e1 e2) t1
+    | WT_Eunop: forall ast_id tb op e,
+        well_typed_expr tb e Tbool ->
+        well_typed_expr tb (Eunop ast_id op e) Tbool.
+
+
+(** ** Well-typed commands *)
+(**
+   two kinds of type checking:
+   - general type checking;
+   - _in/out_ mode checking;
+*)
+Inductive well_typed_stmt: symtb -> stmt  -> Prop :=
+    | WT_Sassign: forall ast_id tb x e t,
+        lookup x tb = Some (Out, t) ->
+        well_typed_expr tb e t ->
+        well_typed_stmt tb ((Sassign ast_id x e))
+    | WT_Sseq: forall ast_id c1 c2 tb,
+        well_typed_stmt tb c1 ->
+        well_typed_stmt tb c2 ->
+        well_typed_stmt tb (Sseq ast_id c1 c2)
+    | WT_Sifthen: forall ast_id tb b c,
+        well_typed_expr tb b Tbool ->
+        well_typed_stmt tb c ->
+        well_typed_stmt tb (Sifthen ast_id b c)
+    | WT_Swhile: forall ast_id tb b c,
+        well_typed_expr tb b Tbool ->
+        well_typed_stmt tb c ->
+        well_typed_stmt tb (Swhile ast_id b c).
+(*    | WT_Sassert: forall ast_id tb e, 
+        well_typed_expr tb e Tbool ->
+        well_typed_stmt tb (Sassert ast_id e) *)
+
+(* =============================== *)
+
+(** * Well-Defined *)
+
+(** basic data structures for well-defined expressions and commands *)
+Inductive init_mode: Type := 
+    | Init: init_mode
+    | Uninit: init_mode.
+
+Definition initializationState: Type := list (idnum * init_mode).
+
+(** basic operators for well-defined expressions and commands *)
+Function fetch2 (x : idnum) (s : initializationState): option init_mode := 
+    match s with 
+    | (y, imode) :: s' =>
+      if beq_nat x y then
+        Some imode
+      else fetch2 x s' 
+    | nil => None
+    end.
+
+Function update2 (s: initializationState) (x : idnum) (v: init_mode): option initializationState := 
+    match s with 
+    | (y, imode) :: s' => 
+      if beq_nat x y then 
+        Some ((y,v)::s') 
+      else 
+        match update2 s' x v with
+        | Some s'' => Some ((y, imode)::s'')
+        | None => None
+        end
+   | nil => None
+   end.
+
+(** ** Well-defined expressions *)
+(**
+    all referenced variables are initialized 
+*)
+Inductive well_defined_expr: initializationState -> expr -> Prop :=
+    | WD_Econst_Int: forall ast_id s n,
+        well_defined_expr s (Econst ast_id (Ointconst n))
+    | WD_Econst_Bool: forall ast_id s b,
+        well_defined_expr s (Econst ast_id (Oboolconst b))
+    | WD_Evar: forall ast_id x s,
+        fetch2 x s = Some Init ->
+        well_defined_expr s (Evar ast_id x)
+    | WD_Ebinop: forall ast_id s op e1 e2,
+        well_defined_expr s e1 ->
+        well_defined_expr s e2 ->
+        well_defined_expr s (Ebinop ast_id op e1 e2)
+    | WD_Eunop: forall ast_id s op e,
+        well_defined_expr s e ->
+        well_defined_expr s (Eunop ast_id op e). 
+
+(*
+Inductive well_defined_expr: stack -> expr -> Prop :=
+    | WD_Econst_Int: forall ast_id s n,
+        well_defined_expr s (Econst ast_id (Ointconst n))
+    | WD_Econst_Bool: forall ast_id s b,
+        well_defined_expr s (Econst ast_id (Oboolconst b))
+    | WD_Evar: forall ast_id x v s,
+        fetch x s = Some v ->
+        well_defined_expr s (Evar ast_id x)
+    | WD_Ebinop: forall ast_id s op e1 e2,
+        well_defined_expr s e1 ->
+        well_defined_expr s e2 ->
+        well_defined_expr s (Ebinop ast_id op e1 e2)
+    | WD_Eunop: forall ast_id s op e,
+        well_defined_expr s e ->
+        well_defined_expr s (Eunop ast_id op e). 
+*)
+
+(** ** Well-defined commands *)
+Inductive well_defined_stmt: initializationState -> stmt -> initializationState -> Prop :=
+    | WD_Sassign: forall ast_id s s' x e,
+        well_defined_expr s e ->
+        update2 s x Init = Some s' ->
+        well_defined_stmt s (Sassign ast_id x e) s'
+    | WD_Sseq: forall ast_id c1 c2 s s' s'',
+        well_defined_stmt s c1 s' ->
+        well_defined_stmt s' c2 s'' ->
+        well_defined_stmt s (Sseq ast_id c1 c2) s''
+    | WD_Sifthen: forall ast_id s s' b c,
+        well_defined_expr s b ->
+        well_defined_stmt s c s' ->
+        well_defined_stmt s (Sifthen ast_id b c) s
+    | WD_Swhile: forall ast_id s s' b c,
+        well_defined_expr s b ->
+        well_defined_stmt s c s' ->
+        well_defined_stmt s (Swhile ast_id b c) s.
+
+(** ** Lemmas about initialization operations *)
+Lemma update2_fetch2: forall istate x m istate',
+    update2 istate x m = Some istate' ->
+    exists m0, fetch2 x istate = Some m0.
+Proof.
+    intros istate x m.
+    functional induction (update2 istate x m);
+    intros istate' h1.
+  - unfold fetch2.
+    rewrite e0.
+    exists imode; auto.
+  - unfold fetch2.
+    rewrite e0.
+    fold fetch2.
+    specialize (IHo _ e1); assumption.
+  - inversion h1.
+  - inversion h1.
+Qed.
+
+Lemma fetch2_update2: forall x istate m0 m,
+    fetch2 x istate = Some m0 ->
+    exists istate', update2 istate x m = Some istate'.
+Proof.
+    intros x istate.
+    functional induction (fetch2 x istate);
+    intros m0 m h1.
+  - unfold update2.
+    rewrite e0.
+    exists ((y, m) :: s'); auto.
+  - unfold update2. 
+    rewrite e0.
+    fold update2.
+    specialize (IHo _ m h1).
+    inversion IHo.
+    rewrite H.
+    exists ((y, imode) :: x0); auto.
+  - inversion h1.
+Qed.
+
+Lemma update2_in: forall istate x m istate' y m',
+    update2 istate x m = Some istate' ->
+    fetch2 y istate = Some m' ->
+    (fetch2 y istate' = Some m) \/ (fetch2 y istate' = Some m').
+Proof.
+    intros istate x m.
+    functional induction (update2 istate x m);
+    intros istate' y0 m' h1 h2.
+  - inversion h1; subst.
+    unfold fetch2.
+    unfold fetch2 in h2.
+    destruct (beq_nat y0 y).
+    + left; auto.
+    + fold fetch2.
+       fold fetch2 in h2.
+       right; assumption.
+  - inversion h1; subst.
+    unfold fetch2.
+    unfold fetch2 in h2.
+    destruct (beq_nat y0 y).
+    + right; assumption.
+    + fold fetch2.
+       fold fetch2 in h2.
+       specialize (IHo _ _ _ e1 h2).
+       assumption.
+  - inversion h1.
+  - inversion h1.
+Qed.
+
+Lemma update2_in1: forall istate x m istate' y m',
+    update2 istate x m = Some istate' ->
+    fetch2 y istate' = Some m' ->
+    (y = x /\ m' = m) \/ (y <> x /\ fetch2 y istate = Some m').
+Proof.
+    intros istate x m.
+    functional induction (update2 istate x m);
+    intros istate' y0 m' h1 h2.
+  - inversion h1; subst.
+    unfold fetch2.
+    unfold fetch2 in h2.
+    remember (beq_nat y0 y) as eq.
+    destruct eq.
+    + left. 
+       inversion h2; subst.
+       apply beq_nat_true in e0.
+       symmetry in Heqeq.
+       apply beq_nat_true in Heqeq.
+       subst. auto.
+    + right. 
+       fold fetch2.
+       fold fetch2 in h2.
+       symmetry in Heqeq.
+       apply beq_nat_true in e0.
+       apply beq_nat_false in Heqeq.
+       subst.
+       split; assumption.
+  - inversion h1; subst.
+    unfold fetch2.
+    unfold fetch2 in h2.
+    remember (beq_nat y0 y) as eq.
+    destruct eq.
+    + right.
+       symmetry in Heqeq.
+       apply beq_nat_false in e0;
+       apply beq_nat_true in Heqeq; subst.
+       split; auto.
+    + fold fetch2.
+       fold fetch2 in h2.
+       specialize (IHo _ _ _ e1 h2).
+       assumption.
+  - inversion h1.
+  - inversion h1.  
+Qed.
+
+Lemma update2_fetch2_new: forall istate x m istate',
+    update2 istate x m = Some istate' ->
+    fetch2 x istate' = Some m.
+Proof.
+    intros istate x m.
+    functional induction (update2 istate x m);
+    intros istate' h1.
+  - inversion h1; subst.
+    unfold fetch2.
+    destruct (beq_nat x y).
+    + auto.
+    + inversion e0.
+  - inversion h1; subst.
+    unfold fetch2.
+    destruct (beq_nat x y).
+    + inversion e0.
+    + fold fetch2.
+       specialize (IHo _ e1).
+       assumption.
+  - inversion h1.
+  - inversion h1.    
+Qed.
+
+Lemma update2_fetch2_old: forall istate x m istate' y,
+    update2 istate x m = Some istate' ->
+    y <> x ->
+    fetch2 y istate' = fetch2 y istate.
+Proof.
+    intros istate x m.
+    functional induction (update2 istate x m);
+    intros istate' y0 h1 h2.
+  - inversion h1; subst.
+    apply beq_nat_true in e0.
+    subst.
+    apply beq_nat_false_iff in h2.
+    unfold fetch2.
+    rewrite h2.
+    fold fetch2.
+    auto.
+  - inversion h1; subst.
+    specialize (IHo _ _ e1 h2).
+    unfold fetch2.
+    destruct (beq_nat y0 y).
+    auto.
+    fold fetch2.
+    assumption.
+  - inversion h1.
+  - inversion h1.    
+Qed.
+
+(** ** Mapping from stack to initialization state *)
+Inductive initializationMap: stack -> initializationState -> Prop :=
+    | IEmpty: initializationMap nil nil 
+    | IList0: forall s ilist x v,
+        v <> Vundef ->
+        initializationMap s ilist ->
+        initializationMap ((x, v)::s) ((x, Init)::ilist)
+    | IList1: forall s ilist x v,
+        v = Vundef ->
+        initializationMap s ilist ->
+        initializationMap ((x, v)::s) ((x, Uninit)::ilist).
+
+(** some useful lemmas *)
+Lemma initializationMap_consistent1: forall s istate x v,
+    initializationMap s istate -> 
+    fetch x s = Some v -> 
+    fetch2 x istate = Some Init.
+Proof.
+    intros s istate x v h1 h2.
+    induction h1.
+      + inversion h2.
+      + unfold fetch in h2. 
+         unfold fetch2.
+         destruct (beq_nat x x0); auto.
+      + unfold fetch in h2.
+         unfold fetch2.
+         destruct (beq_nat x x0);
+         auto.
+         destruct v0.
+         inversion H.
+         inversion h2.
+Qed.
+
+Lemma initializationMap_consistent2: forall s istate x,
+    initializationMap s istate ->
+    fetch2 x istate = Some Init -> 
+    exists v, fetch x s = Some v.
+Proof.
+    intros s istate x h1 h2.
+    induction h1.
+      + inversion h2.
+      + unfold fetch2 in h2. 
+         unfold fetch.
+         destruct (beq_nat x x0); auto.
+         destruct v.
+         exists v; auto.
+         intuition.
+      + unfold fetch2 in h2.
+         unfold fetch.
+         destruct (beq_nat x x0); auto.
+         destruct v.
+         exists v; auto.
+         inversion h2.    
+Qed.
+
+
+Lemma initializationMap_unique: forall s istate istate',
+    initializationMap s istate ->
+    initializationMap s istate' ->
+    istate = istate'.
+Proof.
+    intros s istate istate' h1.
+    generalize istate'. clear istate'.
+    induction h1;
+    intros istate' h2.
+  - inversion h2.
+    auto.
+  - inversion h2; subst.
+    specialize (IHh1 _ H5).
+    subst. auto.
+    intuition.
+  - inversion h2; subst.
+    intuition.
+    specialize (IHh1 _ H5).
+    subst.
+    auto.
+Qed.
+
+Lemma update_consis: forall s istate x v s1 istate1 istate'1,
+    initializationMap s istate -> 
+    update s x (Value v) = Some s1 ->
+    update2 istate x Init = Some istate1 ->
+    initializationMap s1 istate'1 ->
+    istate1 = istate'1.
+Proof.
+    intros s istate x v s1 istate1 istate'1 h1.
+    generalize x v s1 istate1 istate'1.
+    induction h1; intros.
+  - inversion H.
+  - unfold update in H0.
+    unfold update2 in H1.
+    destruct (beq_nat x1 x0).
+    + inversion H0; subst.
+       inversion H1; subst.
+       inversion H2; subst.
+       * specialize (initializationMap_unique _ _ _ h1 H8); intros hz1.
+         subst.
+         auto.
+       * inversion H7.
+    + fold update in H0.
+       fold update2 in H1.
+       remember (update s x1 (Value v1)) as eq1.
+       remember (update2 ilist x1 Init) as eq2.
+       destruct eq1; destruct eq2.
+       * inversion H0; subst; clear H0.
+         inversion H1; subst; clear H1.
+         symmetry in Heqeq1. 
+         symmetry in Heqeq2.
+         inversion H2; subst.
+         specialize (IHh1 _ _ _ _ _ Heqeq1 Heqeq2 H6).
+         subst. auto.
+         intuition.
+       * inversion H1.
+       * inversion H0.
+       * inversion H0.
+  - unfold update in H0.
+    unfold update2 in H1.
+    destruct (beq_nat x1 x0).
+    + inversion H0; subst.
+       inversion H1; subst.
+       inversion H2; subst.
+       * specialize (initializationMap_unique _ _ _ h1 H7); intros hz1.
+         subst.
+         auto.
+       * inversion H6.
+    + fold update in H0.
+       fold update2 in H1.
+       remember (update s x1 (Value v1)) as eq1.
+       remember (update2 ilist x1 Init) as eq2.
+       destruct eq1; destruct eq2.
+       * inversion H0; subst; clear H0.
+         inversion H1; subst; clear H1.
+         symmetry in Heqeq1. 
+         symmetry in Heqeq2.
+         inversion H2; subst.
+         intuition.
+         specialize (IHh1 _ _ _ _ _ Heqeq1 Heqeq2 H5).
+         subst. auto.
+       * inversion H1.
+       * inversion H0.
+       * inversion H0.
+Qed.
+
+
+(* = = = = = = = = = = = = = = = = = = = = = = = = = = = = = = = = *)
+
+(** * Well-Checked *)
+Definition get_ast_id_expr (e: expr): astnum :=
+    match e with
+    | (Econst ast_id n) => ast_id
+    | (Evar ast_id x) => ast_id
+    | (Ebinop ast_id op e1 e2) => ast_id
+    | (Eunop ast_id op e) => ast_id
+    end.
+
+Definition get_ast_id_stmt (c: stmt): astnum :=
+    match c with
+    | (Sassign ast_id x e) => ast_id
+    | (Sseq ast_id c1 c2) => ast_id
+    | (Sifthen ast_id b c) => ast_id
+    | (Swhile ast_id b c) => ast_id
+    end.
+
+(** ast_id for each AST node is unique *)
+Definition max_id := astnum.
+
+Inductive ast_id_inc_expr: expr -> max_id -> Prop :=
+    | Inc_Econst: forall ast_id n,
+        ast_id_inc_expr (Econst ast_id n) ast_id
+    | Inc_Evar: forall ast_id x,
+        ast_id_inc_expr (Evar ast_id x) ast_id
+    | Inc_Ebinop: forall e1 max1 e2 max2 ast_id1 ast_id2 ast_id op,
+        ast_id_inc_expr e1 max1 ->
+        ast_id_inc_expr e2 max2 ->
+        get_ast_id_expr e1 = ast_id1 ->
+        get_ast_id_expr e2 = ast_id2 ->
+        ast_id < ast_id1 ->
+        ast_id < ast_id2 ->
+        max1 < ast_id2 ->
+        ast_id_inc_expr (Ebinop ast_id op e1 e2) max2
+    | Inc_Eunop: forall e max ast_id0 ast_id op,
+        ast_id_inc_expr e max ->
+        get_ast_id_expr e = ast_id0 ->
+        ast_id < ast_id0 ->
+        ast_id_inc_expr (Eunop ast_id op e) max.
+
+Inductive ast_id_inc_stmt: stmt -> max_id -> Prop :=
+    | Inc_Sassign: forall e max ast_id0 ast_id x,
+        ast_id_inc_expr e max ->
+        get_ast_id_expr e = ast_id0 ->
+        ast_id < ast_id0 ->
+        ast_id_inc_stmt (Sassign ast_id x e) max
+    | Inc_Sseq: forall c1 max1 c2 max2 ast_id1 ast_id2 ast_id,
+        ast_id_inc_stmt c1 max1 ->
+        ast_id_inc_stmt c2 max2 ->
+        get_ast_id_stmt c1 = ast_id1 ->
+        get_ast_id_stmt c2 = ast_id2 ->
+        ast_id < ast_id1 ->
+        ast_id < ast_id2 ->
+        max1 < ast_id2 ->
+        ast_id_inc_stmt (Sseq ast_id c1 c2) max2
+    | Inc_Sifthen: forall b max1 c max2 ast_id1 ast_id2 ast_id,
+        ast_id_inc_expr b max1 ->
+        ast_id_inc_stmt c max2 ->
+        get_ast_id_expr b = ast_id1 ->
+        get_ast_id_stmt c = ast_id2 ->
+        ast_id < ast_id1 ->
+        ast_id < ast_id2 ->
+        max1 < ast_id2 ->
+        ast_id_inc_stmt (Sifthen ast_id b c) max2
+    | Inc_Swhile: forall b max1 c max2 ast_id1 ast_id2 ast_id,
+        ast_id_inc_expr b max1 ->
+        ast_id_inc_stmt c max2 ->
+        get_ast_id_expr b = ast_id1 ->
+        get_ast_id_stmt c = ast_id2 ->
+        ast_id < ast_id1 -> 
+        ast_id < ast_id2 -> 
+        max1 < ast_id2 ->
+        ast_id_inc_stmt (Swhile ast_id b c) max2.
+
+
+(** ** Generate the run-time-check flags *)
+
+Definition check_points :=  list (astnum * check_action).
+
+Function fetch_ck (id : astnum) (m : check_points): option check_action := 
+    match m with 
+    | (id0, ck0) :: s0 =>
+      if beq_nat id id0 then
+        Some ck0
+      else 
+        fetch_ck id s0 
+    | nil => None
+    end.
+
+Inductive ast_ids_lt: check_points -> astnum -> Prop := 
+    | lt1: forall ls n ast_id ck,
+        ast_ids_lt ls n ->
+        ast_id < n ->
+        ast_ids_lt ((ast_id, ck) ::ls) n
+    | lt2: forall n,
+        ast_ids_lt nil n.
+
+Lemma ast_ids_lt_trans0: forall ls n n',
+    ast_ids_lt ls n ->
+    n <= n' ->
+    ast_ids_lt ls n'.
+Proof.
+    intros ls n n' h1 h2.
+    induction h1.
+  - constructor.
+    apply IHh1; assumption.
+    intuition.
+  - constructor.    
+Qed.
+
+Lemma ast_ids_lt_trans: forall ls n n',
+    ast_ids_lt ls n ->
+    n < n' ->
+    ast_ids_lt ls n'.
+Proof.
+    intros.
+    eapply ast_ids_lt_trans0.
+    apply H. 
+    intuition.
+Qed.
+
+
+(** *** generate run-time-check flags for expressions *)
+Inductive check_generator_expr: check_points -> expr -> check_points -> Prop :=
+    | CG_Econst: forall ast_id n flag ls,
+        check_flag (Econst ast_id n) flag -> 
+        check_generator_expr ls (Econst ast_id n) ((ast_id, flag ) :: ls)
+    | CG_Evar: forall ast_id x flag ls,
+        check_flag (Evar ast_id x) flag ->
+        check_generator_expr ls (Evar ast_id x) ((ast_id, flag) :: ls)
+    | CG_Ebinop: forall ls e1 ls1 e2 ls2 ast_id op flag,
+        check_generator_expr ls e1 ls1 ->
+        check_generator_expr ls1 e2 ls2 ->
+        check_flag (Ebinop ast_id op e1 e2) flag -> 
+        check_generator_expr ls (Ebinop ast_id op e1 e2) ((ast_id, flag) :: ls2)
+    | CG_Eunop: forall ls e ls1 ast_id op flag,
+        check_generator_expr ls e ls1 ->
+        check_flag (Eunop ast_id op e) flag ->
+        check_generator_expr ls (Eunop ast_id op e) ((ast_id, flag ) :: ls1).
+
+(** *** generate run-time-check flags for statements *)
+(** For the SPARK 2014 subset that we are working on, we only consider the division by zero check and 
+     overflow check. So here, the check for each statement is none, but it is extensible to includes necessary 
+     checks in the statements in the future. 
+ *)
+Inductive check_generator_stmt: check_points -> stmt -> check_points -> Prop :=
+    | CG_Sassign: forall ls1 e ls2 ast_id x,
+        check_generator_expr ls1 e ls2 ->
+        check_generator_stmt ls1 (Sassign ast_id x e) ((ast_id, No_Check) :: ls2)
+    | CG_Sseq: forall ls1 c1 ls2 c2 ls3 ast_id,
+        check_generator_stmt ls1 c1 ls2 ->
+        check_generator_stmt ls2 c2 ls3 ->
+        check_generator_stmt ls1 (Sseq ast_id c1 c2) ((ast_id, No_Check) :: ls3)
+    | CG_Sifthen: forall ls1 b ls2 c ls3 ast_id,
+        check_generator_expr ls1 b ls2 ->
+        check_generator_stmt ls2 c ls3 ->
+        check_generator_stmt ls1 (Sifthen ast_id b c) ((ast_id, No_Check) :: ls3)
+    | CG_Swhile: forall ls1 b ls2 c ls3 ast_id,
+        check_generator_expr ls1 b ls2 ->
+        check_generator_stmt ls2 c ls3 ->        
+        check_generator_stmt ls1 (Swhile ast_id b c) ((ast_id, No_Check) :: ls3).
+
+(** ** Semantics with run-time-checks *)
+Inductive eval_expr_with_checks (cps: check_points): stack -> expr -> return_val -> Prop :=
+    | eval_Const: forall cst v s ast_id,
+        eval_constant cst = v ->
+        eval_expr_with_checks cps s (Econst ast_id cst) v
+    | eval_Var: forall x s v ast_id,
+        fetch x s = Some v ->
+        eval_expr_with_checks cps s (Evar ast_id x) (ValNormal v)
+    | eval_Binop1: forall s e1 ast_id op e2,
+        eval_expr_with_checks cps s e1 ValException ->
+        eval_expr_with_checks cps s (Ebinop ast_id op e1 e2) ValException
+    | eval_Binop2: forall s e1 v1 e2 ast_id op,
+        eval_expr_with_checks cps s e1 (ValNormal v1) ->
+        eval_expr_with_checks cps s e2 ValException ->
+        eval_expr_with_checks cps s (Ebinop ast_id op e1 e2) ValException
+    | eval_Binop3: forall s e1 v1 e2 v2 ck ast_id op,
+        eval_expr_with_checks cps s e1 (ValNormal v1) ->
+        eval_expr_with_checks cps s e2 (ValNormal v2) ->
+        fetch_ck ast_id cps = Some ck -> 
+        do_check (eval_expr_with_checks cps) s ck false ->
+        eval_expr_with_checks cps s (Ebinop ast_id op e1 e2) ValException
+    | eval_Binop4: forall s e1 v1 e2 v2 ck ast_id op v,
+        eval_expr_with_checks cps s e1 (ValNormal v1) ->
+        eval_expr_with_checks cps s e2 (ValNormal v2) ->
+        fetch_ck ast_id cps = Some ck -> 
+        do_check (eval_expr_with_checks cps) s ck true ->
+        eval_binop op (ValNormal v1) (ValNormal v2) = v ->
+        v <> ValAbnormal ->
+        eval_expr_with_checks cps s (Ebinop ast_id op e1 e2) v
+    | eval_Unop1: forall s e ast_id op,
+        eval_expr_with_checks cps s e ValException ->
+        eval_expr_with_checks cps s (Eunop ast_id op e) ValException
+    | eval_Unop2: forall s e v ast_id op v1,
+        eval_expr_with_checks cps s e (ValNormal v) ->
+        eval_unop op (ValNormal v) = v1 ->
+        v1 <> ValAbnormal ->
+        eval_expr_with_checks cps s (Eunop ast_id op e) v1.
+
+
+Inductive eval_stmt_with_checks (cps: check_points): stack -> stmt -> state -> Prop :=
+    | eval_Assign1: forall s e ast_id x,
+        eval_expr_with_checks cps s e ValException ->
+        eval_stmt_with_checks cps s (Sassign ast_id x e) SException
+    | eval_Assign2: forall s e v x s1 ast_id,
+        eval_expr_with_checks cps s e (ValNormal v) ->
+        update s x (Value v) = Some s1 -> (* needs the type check on both sides *)
+        eval_stmt_with_checks cps s (Sassign ast_id x e) (SNormal s1)
+    | eval_Seq1: forall s c1 ast_id c2,
+        eval_stmt_with_checks cps s c1 SException ->
+        eval_stmt_with_checks cps s (Sseq ast_id c1 c2) SException
+    | eval_Seq2: forall ast_id s s1 s2 c1 c2,
+        eval_stmt_with_checks cps s c1 (SNormal s1) ->
+        eval_stmt_with_checks cps s1 c2 s2 ->
+        eval_stmt_with_checks cps s (Sseq ast_id c1 c2) s2
+    | eval_Ifthen: forall s b ast_id c,
+        eval_expr_with_checks cps s b ValException ->
+        eval_stmt_with_checks cps s (Sifthen ast_id b c) SException
+    | eval_Ifthen_True: forall s b c s1 ast_id,
+        eval_expr_with_checks cps s b (ValNormal (Bool true)) ->
+        eval_stmt_with_checks cps s c s1 ->
+        eval_stmt_with_checks cps s (Sifthen ast_id b c) s1
+    | eval_Ifthen_False: forall s b ast_id c,
+        eval_expr_with_checks cps s b (ValNormal (Bool false)) ->
+        eval_stmt_with_checks cps s (Sifthen ast_id b c) (SNormal s)
+    | eval_While: forall s b ast_id c,
+        eval_expr_with_checks cps s b ValException ->
+        eval_stmt_with_checks cps s (Swhile ast_id b c) SException
+    | eval_While_True1: forall s b c ast_id,
+        eval_expr_with_checks cps s b (ValNormal (Bool true)) ->
+        eval_stmt_with_checks cps s c SException ->
+        eval_stmt_with_checks cps s (Swhile ast_id b c) SException
+    | eval_While_True2: forall s b c s1 ast_id s2,
+        eval_expr_with_checks cps s b (ValNormal (Bool true)) ->
+        eval_stmt_with_checks cps s c (SNormal s1) ->
+        eval_stmt_with_checks cps s1 (Swhile ast_id b c) s2 ->
+        eval_stmt_with_checks cps s (Swhile ast_id b c) s2
+    | eval_While_False: forall s b ast_id c,
+        eval_expr_with_checks cps s b (ValNormal (Bool false)) ->
+        eval_stmt_with_checks cps s (Swhile ast_id b c) (SNormal s).
+
+
+(*
+(** ** Semantics: run-time-check never fails *)
+Inductive check_never_fail_expr: stack -> expr -> check_points -> Prop :=
+    | CNF_Econst: forall s ast_id n cps,
+        check_never_fail_expr s (Econst ast_id n) cps
+    | CNF_Evar: forall s ast_id x cps,  
+        check_never_fail_expr s (Evar ast_id x) cps
+    | CNF_Ebinop: forall s e1 cps e2 ast_id ck op,
+        check_never_fail_expr s e1 cps ->
+        check_never_fail_expr s e2 cps ->
+        (fetch_ck ast_id cps = Some ck -> run_time_check eval_expr s (check_expr ck) true) ->
+        check_never_fail_expr s (Ebinop ast_id op e1 e2) cps
+    | CNF_Eunop: forall s e cps ast_id ck op,
+        check_never_fail_expr s e cps ->
+        (fetch_ck ast_id cps = Some ck -> run_time_check eval_expr s (check_expr ck) true) ->
+        check_never_fail_expr s (Eunop ast_id op e) cps.
+
+Inductive check_never_fail_stmt: stack -> stmt -> check_points -> Prop :=
+    | CNF_Sassign: forall s e cps ast_id x,
+        check_never_fail_expr s e cps ->
+(*        (fetch_ck ast_id cps = Some ck -> run_time_check eval_expr s (check_expr ck) true) -> *)
+        check_never_fail_stmt s (Sassign ast_id x e) cps
+    | CNF_Sseq: forall s c1 cps s' c2 ast_id,
+        check_never_fail_stmt s c1 cps->
+        eval_stmt s c1 (SNormal s') -> 
+        check_never_fail_stmt s' c2 cps ->
+        check_never_fail_stmt s (Sseq ast_id c1 c2)  cps   
+    | CNF_Sifthen_False: forall s b cps ast_id c,
+        check_never_fail_expr s b cps ->
+        eval_expr s b (ValNormal (Bool false)) ->
+        check_never_fail_stmt s (Sifthen ast_id b c) cps
+    | CNF_Sifthen_True: forall s b cps c ast_id,
+        check_never_fail_expr s b cps ->
+        eval_expr s b (ValNormal (Bool true)) ->
+        check_never_fail_stmt s c cps ->
+        check_never_fail_stmt s (Sifthen ast_id b c) cps
+    | CNF_Swhile_False: forall s b cps c ast_id,
+        check_never_fail_expr s b cps ->
+        eval_expr s b (ValNormal (Bool false)) ->
+        check_never_fail_stmt s (Swhile ast_id b c) cps
+    | CNF_Swhile: forall s b cps c s' ast_id,
+        check_never_fail_expr s b cps ->
+        eval_expr s b (ValNormal (Bool true)) ->     
+        check_never_fail_stmt s c cps ->
+        eval_stmt s c (SNormal s') ->
+        check_never_fail_stmt s' (Swhile ast_id b c) cps -> 
+        check_never_fail_stmt s (Swhile ast_id b c) cps.
+*)
+
+(** some basic lemmas *)
+Lemma eval_expr_with_checks_state: forall ls s e v,
+    eval_expr_with_checks ls s e v ->
+    (exists v0, v = ValNormal v0) \/ v = ValException.
+Proof.
+    intros.
+    induction H;
+    try match goal with
+    | [ |- (exists v0 : value, ValNormal v = ValNormal v0) \/ _ ] => left; exists v; reflexivity
+    | [ |- _ \/ ?A = ?A ] => right; reflexivity
+    end.
+  - destruct cst; simpl in H; rewrite <- H;
+    left; 
+    [exists (Int z) | exists (Bool b)]; reflexivity.
+  - destruct v.
+    left; exists v; reflexivity.
+    right; reflexivity.
+    intuition.
+  - destruct v1.
+    left; exists v0; reflexivity.
+    right; reflexivity.
+    intuition.    
+Qed.
+
+Lemma eval_expr_with_checks_unique: forall ls s e v1 v2,
+    eval_expr_with_checks ls s e (ValNormal v1) ->
+    eval_expr_with_checks ls s e (ValNormal v2) ->
+    v1 = v2.
+Proof.
+    induction e;
+    intros v1 v2 h1 h2;
+    inversion h1; subst;
+    inversion h2; subst.
+  - rewrite H3 in H4.
+    inversion H4; subst;
+    reflexivity.
+  - rewrite H1 in H2; inversion H2; subst; 
+    reflexivity.
+  - specialize (IHe1 _ _ H3 H5).
+    specialize (IHe2 _ _ H4 H7). subst.
+    rewrite H15 in H9; inversion H9; subst.
+    reflexivity.
+  - specialize (IHe _ _ H1 H2).
+    subst. 
+    destruct op0, op.
+    rewrite H6 in H3; inversion H3; subst;
+    auto.
+Qed.
+
+(*
+Lemma eval_expr_with_checks_unique: forall ls s e v1 v2,
+    eval_expr_with_checks ls s e v1 ->
+    eval_expr_with_checks ls s e v2 ->
+    v1 = v2.
+Proof.
+    induction e;
+    intros v1 v2 h1 h2.
+  - inversion h1; subst. 
+    inversion h2; subst.
+    reflexivity.
+  - inversion h1; subst. 
+    inversion h2; subst.
+    rewrite H3 in H4; inversion H4; subst; reflexivity.
+  - inversion h1; subst.
+    inversion h2; subst; auto;
+    repeat match goal with
+    | [ h1:  forall v1 v2,
+               eval_expr_with_checks ?ls ?s ?e v1 ->
+               eval_expr_with_checks ?ls ?s ?e v2 -> v1 = v2, 
+        h2: eval_expr_with_checks ?ls ?s ?e ?x,
+        h3: eval_expr_with_checks ?ls ?s ?e ?y |- _ ] => specialize (h1 _ _ h2 h3); inversion h1; subst
+    end; auto.
+    rewrite H7 in H10. inversion H10; subst. 
+    clear IHe2 IHe1 H6 H4 H10.
+    
+    inversion H8; subst.
+    inversion H8; subst.
+    inversion H12; subst.   
+    
+    - inversion h1; subst;
+      inversion h2; subst; auto;
+      match goal with
+      | [ h1:  forall v1 v2,
+               eval_expr_with_checks ?ls ?s ?e v1 ->
+               eval_expr_with_checks ?ls ?s ?e v2 -> v1 = v2, 
+        h2: eval_expr_with_checks ?ls ?s ?e ?x,
+        h3: eval_expr_with_checks ?ls ?s ?e ?y |- _ ] => specialize (h1 _ _ h2 h3); inversion h1; subst
+    end; auto.
+    destruct op, op0; auto.
+Qed.
+*)
+
+Lemma ast_id_bound_expr: forall e max,
+    ast_id_inc_expr e max ->
+    get_ast_id_expr e <= max.
+Proof.
+    intros e max h.
+    induction h; simpl; intuition.
+Qed.
+
+
+Lemma ast_id_max_expr: forall e max cks0 cks,
+    ast_id_inc_expr e max ->
+    check_generator_expr cks0 e cks ->
+    ast_ids_lt cks0 (get_ast_id_expr e) ->
+    ast_ids_lt cks (max + 1).
+Proof.
+    intros e max cks0 cks h1.
+    revert cks0 cks.
+    induction h1;
+    intros cks0 cks h2 h3;
+    simpl in h3; inversion h2; subst.
+  - constructor.
+    apply ast_ids_lt_trans with (n := ast_id); intuition.
+    intuition.
+  - constructor.
+    apply ast_ids_lt_trans with (n := ast_id); intuition.
+    intuition.
+  - specialize (ast_ids_lt_trans _ _ _ h3 H1); intros hz1.
+    specialize (ast_ids_lt_trans _ _ _ h3 H2); intros hz2.
+    specialize (IHh1_1 _ _ H10 hz1).
+    assert(hz: max1 + 1 <= get_ast_id_expr e2); intuition.
+    specialize (ast_ids_lt_trans0 _ _ _ IHh1_1 hz); intros hz3.
+    specialize (IHh1_2 _ _ H11 hz3).
+    constructor.
+    + assumption.
+    + specialize (ast_id_bound_expr _ _ h1_2); intros hz4.
+       intuition.
+  - specialize (ast_ids_lt_trans _ _ _ h3 H0); intros hz1.
+    specialize (IHh1 _ _ H4 hz1).
+    constructor.
+    + assumption.
+    + specialize (ast_id_bound_expr _ _ h1); intros hz2.
+       intuition.
+Qed.
+
+Lemma ast_id_bound_stmt: forall c max,
+    ast_id_inc_stmt c max ->
+    get_ast_id_stmt c <= max.
+Proof.
+    intros c max h.
+    induction h; simpl; intuition.
+    specialize (ast_id_bound_expr _ _ H); intros hz1.
+    intuition.    
+Qed.
+
+
+Lemma ast_id_max_stmt: forall c max cks0 cks1,
+    ast_id_inc_stmt c max ->
+    check_generator_stmt cks0 c cks1 ->
+    ast_ids_lt cks0 (get_ast_id_stmt c) ->
+    ast_ids_lt cks1 (max + 1).
+Proof.
+    intros c max cks0 cks1 h1.
+    revert cks0 cks1.
+    induction h1;
+    intros cks0 cks1 h2 h3;
+    simpl in h3; inversion h2; subst.
+  - specialize (ast_ids_lt_trans _ _ _ h3 H1); intros hz1.
+    specialize (ast_id_max_expr _ _ _ _ H H7 hz1); intros hz2.
+    specialize (ast_id_bound_expr _ _ H); intros hz3.
+    constructor; intuition.
+  - specialize (ast_ids_lt_trans _ _ _ h3 H1); intros hz1.
+    specialize (IHh1_1 _ _ H9 hz1).
+    assert (hz: max1 + 1 <= get_ast_id_stmt c2); intuition.
+    specialize (ast_ids_lt_trans0 _ _ _ IHh1_1 hz); intros hz2.
+    specialize (IHh1_2 _ _ H10 hz2).
+    constructor. assumption.
+    specialize (ast_id_bound_stmt _ _ h1_2); intros hz3.
+    intuition.
+  - specialize (ast_ids_lt_trans _ _ _ h3 H2); intros hz1.
+    specialize (ast_id_max_expr _ _ _ _ H H10 hz1); intros hz2.
+    assert (hz: max1 + 1 <= get_ast_id_stmt c); intuition.
+    specialize (ast_ids_lt_trans0 _ _ _ hz2 hz); intros hz3.
+    specialize (IHh1 _ _ H11 hz3).
+    constructor. assumption.
+    specialize (ast_id_bound_stmt _ _ h1); intros hz4.
+    intuition.
+  - specialize (ast_ids_lt_trans _ _ _ h3 H2); intros hz1.
+    specialize (ast_id_max_expr _ _ _ _ H H10 hz1); intros hz2.
+    assert (hz: max1 + 1 <= get_ast_id_stmt c); intuition.
+    specialize (ast_ids_lt_trans0 _ _ _ hz2 hz); intros hz3.
+    specialize (IHh1 _ _ H11 hz3).
+    constructor. assumption.
+    specialize (ast_id_bound_stmt _ _ h1); intros hz4.
+    intuition.
+Qed.
+
+
+
+
+
+
+
+
+
+
+
+
+
+
